<?xml version="1.0"?>
<rdf:RDF xmlns="http://eao.onl/ontologies/eao.owl#"
     xml:base="http://eao.onl/ontologies/eao.owl"
     xmlns:dc="http://purl.org/dc/elements/1.1/"
     xmlns:eao="http://eao.onl/ontologies/eao.owl#"
     xmlns:obo="http://purl.obolibrary.org/obo/"
     xmlns:owl="http://www.w3.org/2002/07/owl#"
     xmlns:rdf="http://www.w3.org/1999/02/22-rdf-syntax-ns#"
     xmlns:xml="http://www.w3.org/XML/1998/namespace"
     xmlns:xsd="http://www.w3.org/2001/XMLSchema#"
     xmlns:foaf="http://xmlns.com/foaf/0.1/"
     xmlns:rdfs="http://www.w3.org/2000/01/rdf-schema#"
     xmlns:terms="http://purl.org/dc/terms/"
     xmlns:oboInOwl="http://www.geneontology.org/formats/oboInOwl#"
     xmlns:CommonCoreOntologies="http://www.ontologyrepository.com/CommonCoreOntologies/">
    <owl:Ontology rdf:about="http://eao.onl/ontologies/eao.owl">
        <owl:versionIRI rdf:resource="http://eao.onl/ontologies/eao.owl/0.1"/>
        <owl:imports rdf:resource="http://purl.obolibrary.org/obo/bfo/2.0/bfo.owl"/>
        <owl:imports rdf:resource="http://www.ontologyrepository.com/CommonCoreOntologies/Mid/2021-03-01/EventOntology"/>
        <owl:imports rdf:resource="http://www.ontologyrepository.com/CommonCoreOntologies/Mid/2021-03-01/ExtendedRelationOntology"/>
        <rdfs:comment xml:lang="en">This ontology is designed to represent an enterprise archtiecture, inspired by the Archimate framework.</rdfs:comment>
        <rdfs:label xml:lang="en">Enterprise Architecture Ontology</rdfs:label>
        <owl:versionInfo xml:lang="en">Version 0.1</owl:versionInfo>
    </owl:Ontology>
    


    <!-- 
    ///////////////////////////////////////////////////////////////////////////////////////
    //
    // Annotation properties
    //
    ///////////////////////////////////////////////////////////////////////////////////////
     -->

    


    <!-- http://eao.onl/ontologies/eao.owl#archimate_relationship -->

    <owl:AnnotationProperty rdf:about="http://eao.onl/ontologies/eao.owl#archimate_relationship"/>
    


    <!-- 
    ///////////////////////////////////////////////////////////////////////////////////////
    //
    // Object Properties
    //
    ///////////////////////////////////////////////////////////////////////////////////////
     -->

    


    <!-- http://eao.onl/ontologies/eao.owl#accesses -->

    <owl:ObjectProperty rdf:about="http://eao.onl/ontologies/eao.owl#accesses">
        <rdfs:subPropertyOf rdf:resource="http://www.w3.org/2002/07/owl#topObjectProperty"/>
        <owl:inverseOf rdf:resource="http://eao.onl/ontologies/eao.owl#isAccessedBy"/>
        <archimate_relationship xml:lang="en">access</archimate_relationship>
        <dc:source xml:lang="en">https://pubs.opengroup.org/architecture/archimate3-doc/chap05.html</dc:source>
        <rdfs:comment xml:lang="en">Represents the ability of behavior and active structure elements to observe or act upon passive structure elements.

The access relationship indicates that a process, function, interaction, service, or event “does something” with a passive structure element; e.g., create a new object, read data from the object, write or modify the object data, or delete the object. The relationship can also be used to indicate that the object is just associated with the behavior; e.g., it models the information that comes with an event, or the information that is made available as part of a service. The arrow head, if present, indicates the creation, change, or usage of passive structure elements. The access relationship should not be confused with the UML dependency relationship, which uses a similar notation.</rdfs:comment>
        <rdfs:label xml:lang="en">accesses</rdfs:label>
    </owl:ObjectProperty>
    


    <!-- http://eao.onl/ontologies/eao.owl#aggregates -->

    <owl:ObjectProperty rdf:about="http://eao.onl/ontologies/eao.owl#aggregates">
        <rdfs:subPropertyOf rdf:resource="http://purl.obolibrary.org/obo/RO_0001019"/>
        <archimate_relationship xml:lang="en">aggregation</archimate_relationship>
        <dc:source xml:lang="en">https://pubs.opengroup.org/architecture/archimate3-doc/chap05.html</dc:source>
        <rdfs:comment xml:lang="en">Represents that an element combines one or more other concepts. Aggregation does not imply an existence dependency between the aggregating and aggregated concepts. If an aggregation parent is deleted, its children still exist.</rdfs:comment>
        <rdfs:label xml:lang="en">aggregates</rdfs:label>
    </owl:ObjectProperty>
    


    <!-- http://eao.onl/ontologies/eao.owl#create -->

    <owl:ObjectProperty rdf:about="http://eao.onl/ontologies/eao.owl#create">
        <rdfs:subPropertyOf rdf:resource="http://eao.onl/ontologies/eao.owl#accesses"/>
        <rdfs:label xml:lang="en">create</rdfs:label>
    </owl:ObjectProperty>
    


    <!-- http://eao.onl/ontologies/eao.owl#delete -->

    <owl:ObjectProperty rdf:about="http://eao.onl/ontologies/eao.owl#delete">
        <rdfs:subPropertyOf rdf:resource="http://eao.onl/ontologies/eao.owl#accesses"/>
        <rdfs:label xml:lang="en">delete</rdfs:label>
    </owl:ObjectProperty>
    


    <!-- http://eao.onl/ontologies/eao.owl#flowsFrom -->

    <owl:ObjectProperty rdf:about="http://eao.onl/ontologies/eao.owl#flowsFrom">
        <rdfs:subPropertyOf rdf:resource="http://www.w3.org/2002/07/owl#topObjectProperty"/>
        <owl:inverseOf rdf:resource="http://eao.onl/ontologies/eao.owl#flowsTo"/>
        <rdfs:label xml:lang="en">flows from</rdfs:label>
    </owl:ObjectProperty>
    


    <!-- http://eao.onl/ontologies/eao.owl#flowsTo -->

    <owl:ObjectProperty rdf:about="http://eao.onl/ontologies/eao.owl#flowsTo">
        <rdfs:subPropertyOf rdf:resource="http://www.w3.org/2002/07/owl#topObjectProperty"/>
        <dc:source xml:lang="en">https://pubs.opengroup.org/architecture/archimate3-doc/chap05.html</dc:source>
        <rdfs:comment xml:lang="en">Represents transfer from one element to another.</rdfs:comment>
        <rdfs:label xml:lang="en">flows to</rdfs:label>
    </owl:ObjectProperty>
    


    <!-- http://eao.onl/ontologies/eao.owl#hasArchitecture -->

    <owl:ObjectProperty rdf:about="http://eao.onl/ontologies/eao.owl#hasArchitecture">
        <rdfs:subPropertyOf rdf:resource="http://www.w3.org/2002/07/owl#topObjectProperty"/>
        <rdfs:label>has architecture</rdfs:label>
    </owl:ObjectProperty>
    


    <!-- http://eao.onl/ontologies/eao.owl#hasConventionColor -->

    <owl:ObjectProperty rdf:about="http://eao.onl/ontologies/eao.owl#hasConventionColor">
        <rdfs:label>has convention color</rdfs:label>
    </owl:ObjectProperty>
    


    <!-- http://eao.onl/ontologies/eao.owl#hasConventionShape -->

    <owl:ObjectProperty rdf:about="http://eao.onl/ontologies/eao.owl#hasConventionShape">
        <rdfs:subPropertyOf rdf:resource="http://www.w3.org/2002/07/owl#topObjectProperty"/>
        <rdfs:label>has convention shape</rdfs:label>
    </owl:ObjectProperty>
    


    <!-- http://eao.onl/ontologies/eao.owl#hasGeneralization -->

    <owl:ObjectProperty rdf:about="http://eao.onl/ontologies/eao.owl#hasGeneralization">
        <rdfs:subPropertyOf rdf:resource="http://www.w3.org/2002/07/owl#topObjectProperty"/>
        <owl:inverseOf rdf:resource="http://eao.onl/ontologies/eao.owl#hasSpecialization"/>
        <rdfs:label xml:lang="en">has generalization</rdfs:label>
    </owl:ObjectProperty>
    


    <!-- http://eao.onl/ontologies/eao.owl#hasSpecialization -->

    <owl:ObjectProperty rdf:about="http://eao.onl/ontologies/eao.owl#hasSpecialization">
        <dc:source xml:lang="en">https://pubs.opengroup.org/architecture/archimate3-doc/chap05.html</dc:source>
        <rdfs:comment xml:lang="en">Represents that an element is a particular kind of another element.</rdfs:comment>
        <rdfs:label xml:lang="en">has specialization</rdfs:label>
    </owl:ObjectProperty>
    


    <!-- http://eao.onl/ontologies/eao.owl#influences -->

    <owl:ObjectProperty rdf:about="http://eao.onl/ontologies/eao.owl#influences">
        <owl:inverseOf rdf:resource="http://eao.onl/ontologies/eao.owl#isInfluencedBy"/>
        <archimate_relationship xml:lang="en">influence</archimate_relationship>
        <CommonCoreOntologies:example_of_usage xml:lang="en">“Assign Personal Assistant” positively influences “Reduce Workload Of Employees”, but has a negative influence on “Decrease Costs”.</CommonCoreOntologies:example_of_usage>
        <rdfs:comment xml:lang="en">Represents that an element affects the implementation or achievement of some motivation element.

The influence relationship is used to describe that some architectural element influences achievement or implementation of a motivation element, such as a goal or a principle. In general, a motivation element is realized to a certain degree. For example, consistently satisfying the principle “serve customers wherever they are” will help to make the goal “increase market share” come true. In other words, the principle contributes to the goal. In turn, to implement the principle “serve customers wherever they are”, it may be useful to impose a requirement of “24x7 web availability” on some customer-facing application component. This can be modeled as a requirement that has an influence on that principle, and as an application component that in turn influences the requirement. Consistently modeling these dependencies with an influence relationship yields a traceable motivational path that explains why, in this example, a certain application component contributes to the corporate goal to “increase market share”. This kind of traceability supports measuring the results of Enterprise Architecture, and provides valuable information to, for example, change impact assessments.</rdfs:comment>
        <rdfs:label xml:lang="en">influences</rdfs:label>
    </owl:ObjectProperty>
    


    <!-- http://eao.onl/ontologies/eao.owl#isAccessedBy -->

    <owl:ObjectProperty rdf:about="http://eao.onl/ontologies/eao.owl#isAccessedBy">
        <rdfs:subPropertyOf rdf:resource="http://www.w3.org/2002/07/owl#topObjectProperty"/>
        <rdfs:label xml:lang="en">is accessed by</rdfs:label>
    </owl:ObjectProperty>
    


    <!-- http://eao.onl/ontologies/eao.owl#isAssignedTo -->

    <owl:ObjectProperty rdf:about="http://eao.onl/ontologies/eao.owl#isAssignedTo">
        <rdfs:subPropertyOf rdf:resource="http://www.w3.org/2002/07/owl#topObjectProperty"/>
        <archimate_relationship xml:lang="en">assignment</archimate_relationship>
        <dc:source xml:lang="en">https://pubs.opengroup.org/architecture/archimate3-doc/chap05.html</dc:source>
        <rdfs:comment xml:lang="en">Represents the allocation of responsibility, performance of behavior, storage, or execution. Links active structure elements with units of behavior that are performed by them.</rdfs:comment>
        <rdfs:label xml:lang="en">is assigned to</rdfs:label>
    </owl:ObjectProperty>
    


    <!-- http://eao.onl/ontologies/eao.owl#isComposedOf -->

    <owl:ObjectProperty rdf:about="http://eao.onl/ontologies/eao.owl#isComposedOf">
        <rdfs:subPropertyOf rdf:resource="http://purl.obolibrary.org/obo/RO_0001019"/>
        <archimate_relationship xml:lang="en">composition</archimate_relationship>
        <dc:source xml:lang="en">https://pubs.opengroup.org/architecture/archimate3-doc/chap05.html</dc:source>
        <rdfs:comment xml:lang="en">Represents that an element consists of one or more other concepts.  Composition is a whole/part relationship that expresses an existence dependency: if a composite is deleted, its parts are (normally) deleted as well.</rdfs:comment>
        <rdfs:label xml:lang="en">is composed of</rdfs:label>
    </owl:ObjectProperty>
    


    <!-- http://eao.onl/ontologies/eao.owl#isInfluencedBy -->

    <owl:ObjectProperty rdf:about="http://eao.onl/ontologies/eao.owl#isInfluencedBy">
        <rdfs:label xml:lang="en">is influenced by</rdfs:label>
    </owl:ObjectProperty>
    


    <!-- http://eao.onl/ontologies/eao.owl#isServedBy -->

    <owl:ObjectProperty rdf:about="http://eao.onl/ontologies/eao.owl#isServedBy">
        <rdfs:subPropertyOf rdf:resource="http://www.w3.org/2002/07/owl#topObjectProperty"/>
        <owl:inverseOf rdf:resource="http://eao.onl/ontologies/eao.owl#serves"/>
        <rdfs:label xml:lang="en">is served by</rdfs:label>
    </owl:ObjectProperty>
    


    <!-- http://eao.onl/ontologies/eao.owl#isTriggeredBy -->

    <owl:ObjectProperty rdf:about="http://eao.onl/ontologies/eao.owl#isTriggeredBy">
        <rdfs:subPropertyOf rdf:resource="http://www.w3.org/2002/07/owl#topObjectProperty"/>
        <owl:inverseOf rdf:resource="http://eao.onl/ontologies/eao.owl#triggers"/>
        <rdfs:label xml:lang="en">is triggered by</rdfs:label>
    </owl:ObjectProperty>
    


    <!-- http://eao.onl/ontologies/eao.owl#is_associated_with -->

    <owl:ObjectProperty rdf:about="http://eao.onl/ontologies/eao.owl#is_associated_with">
        <archimate_relationship xml:lang="en">association</archimate_relationship>
        <rdfs:comment xml:lang="en">Represents an unspecified relationship, or one that is not represented by another ArchiMate relationship</rdfs:comment>
        <rdfs:label xml:lang="en">is associated with</rdfs:label>
    </owl:ObjectProperty>
    


    <!-- http://eao.onl/ontologies/eao.owl#negatively_influences -->

    <owl:ObjectProperty rdf:about="http://eao.onl/ontologies/eao.owl#negatively_influences">
        <rdfs:subPropertyOf rdf:resource="http://eao.onl/ontologies/eao.owl#influences"/>
        <rdfs:label xml:lang="en">negatively influences</rdfs:label>
    </owl:ObjectProperty>
    


    <!-- http://eao.onl/ontologies/eao.owl#positively_influences -->

    <owl:ObjectProperty rdf:about="http://eao.onl/ontologies/eao.owl#positively_influences">
        <rdfs:subPropertyOf rdf:resource="http://eao.onl/ontologies/eao.owl#influences"/>
        <rdfs:label xml:lang="en">positively influences</rdfs:label>
    </owl:ObjectProperty>
    


    <!-- http://eao.onl/ontologies/eao.owl#read -->

    <owl:ObjectProperty rdf:about="http://eao.onl/ontologies/eao.owl#read">
        <rdfs:subPropertyOf rdf:resource="http://eao.onl/ontologies/eao.owl#accesses"/>
        <rdfs:label xml:lang="en">read</rdfs:label>
    </owl:ObjectProperty>
    


    <!-- http://eao.onl/ontologies/eao.owl#serves -->

    <owl:ObjectProperty rdf:about="http://eao.onl/ontologies/eao.owl#serves">
        <rdfs:subPropertyOf rdf:resource="http://www.w3.org/2002/07/owl#topObjectProperty"/>
        <archimate_relationship xml:lang="en">serving</archimate_relationship>
        <dc:source xml:lang="en">https://pubs.opengroup.org/architecture/archimate3-doc/chap05.html</dc:source>
        <CommonCoreOntologies:example_of_usage xml:lang="en">a service serves a user</CommonCoreOntologies:example_of_usage>
        <rdfs:comment xml:lang="en">Represents that an element provides its functionality to another element.</rdfs:comment>
        <rdfs:label xml:lang="en">serves</rdfs:label>
    </owl:ObjectProperty>
    


    <!-- http://eao.onl/ontologies/eao.owl#triggers -->

    <owl:ObjectProperty rdf:about="http://eao.onl/ontologies/eao.owl#triggers">
        <rdfs:subPropertyOf rdf:resource="http://www.w3.org/2002/07/owl#topObjectProperty"/>
        <dc:source xml:lang="en">https://pubs.opengroup.org/architecture/archimate3-doc/chap05.html</dc:source>
        <rdfs:comment xml:lang="en">Represents a temporal or causal relationship between elements.</rdfs:comment>
        <rdfs:label xml:lang="en">triggers</rdfs:label>
    </owl:ObjectProperty>
    


    <!-- http://eao.onl/ontologies/eao.owl#update -->

    <owl:ObjectProperty rdf:about="http://eao.onl/ontologies/eao.owl#update">
        <rdfs:subPropertyOf rdf:resource="http://eao.onl/ontologies/eao.owl#accesses"/>
        <CommonCoreOntologies:alternative_label xml:lang="en">modify</CommonCoreOntologies:alternative_label>
        <CommonCoreOntologies:alternative_label xml:lang="en">write</CommonCoreOntologies:alternative_label>
        <rdfs:label xml:lang="en">update</rdfs:label>
    </owl:ObjectProperty>
    


    <!-- http://purl.obolibrary.org/obo/BFO_0000055 -->

    <rdf:Description rdf:about="http://purl.obolibrary.org/obo/BFO_0000055">
        <rdfs:subPropertyOf rdf:resource="http://www.w3.org/2002/07/owl#topObjectProperty"/>
        <archimate_relationship xml:lang="en">realization</archimate_relationship>
        <dc:source xml:lang="en">https://pubs.opengroup.org/architecture/archimate3-doc/chap05.html</dc:source>
    </rdf:Description>
    


    <!-- 
    ///////////////////////////////////////////////////////////////////////////////////////
    //
    // Classes
    //
    ///////////////////////////////////////////////////////////////////////////////////////
     -->

    


    <!-- http://eao.onl/ontologies/eao.owl#abstract -->

    <owl:Class rdf:about="http://eao.onl/ontologies/eao.owl#abstract">
        <rdfs:subClassOf rdf:resource="http://eao.onl/ontologies/eao.owl#aspect"/>
        <rdfs:subClassOf>
            <owl:Restriction>
                <owl:onProperty rdf:resource="http://eao.onl/ontologies/eao.owl#hasConventionColor"/>
                <owl:allValuesFrom rdf:resource="http://eao.onl/ontologies/eao.owl#white"/>
            </owl:Restriction>
        </rdfs:subClassOf>
        <dc:source xml:lang="en">https://pubs.opengroup.org/architecture/archimate3-doc/chap03.html</dc:source>
        <rdfs:comment xml:lang="en">non-instantiable, used only in the metamodel</rdfs:comment>
        <rdfs:label xml:lang="en">abstract</rdfs:label>
    </owl:Class>
    


    <!-- http://eao.onl/ontologies/eao.owl#active_structure_aspect -->

    <owl:Class rdf:about="http://eao.onl/ontologies/eao.owl#active_structure_aspect">
        <rdfs:subClassOf rdf:resource="http://eao.onl/ontologies/eao.owl#aspect"/>
        <rdfs:subClassOf>
            <owl:Restriction>
                <owl:onProperty rdf:resource="http://eao.onl/ontologies/eao.owl#hasConventionColor"/>
                <owl:allValuesFrom rdf:resource="http://eao.onl/ontologies/eao.owl#dark_grey"/>
            </owl:Restriction>
        </rdfs:subClassOf>
        <dc:source xml:lang="en">https://pubs.opengroup.org/architecture/archimate3-doc/chap03.html</dc:source>
        <rdfs:comment xml:lang="en">represents the structural elements (the business actors, application components, and devices that display actual behavior; i.e., the “subjects” of activity)</rdfs:comment>
        <rdfs:label xml:lang="en">active structure aspect</rdfs:label>
    </owl:Class>
    


    <!-- http://eao.onl/ontologies/eao.owl#active_structure_element -->

    <owl:Class rdf:about="http://eao.onl/ontologies/eao.owl#active_structure_element">
        <rdfs:subClassOf rdf:resource="http://eao.onl/ontologies/eao.owl#structure_element"/>
        <owl:disjointWith rdf:resource="http://eao.onl/ontologies/eao.owl#passive_structure_element"/>
        <dc:source xml:lang="en">https://pubs.opengroup.org/architecture/archimate3-doc/chap04.html</dc:source>
        <rdfs:comment xml:lang="en">Active structure elements are the subjects that can perform behavior</rdfs:comment>
        <rdfs:label xml:lang="en">active structure element</rdfs:label>
    </owl:Class>
    


    <!-- http://eao.onl/ontologies/eao.owl#application_layer -->

    <owl:Class rdf:about="http://eao.onl/ontologies/eao.owl#application_layer">
        <rdfs:subClassOf rdf:resource="http://eao.onl/ontologies/eao.owl#layer"/>
        <rdfs:subClassOf>
            <owl:Restriction>
                <owl:onProperty rdf:resource="http://eao.onl/ontologies/eao.owl#hasConventionColor"/>
                <owl:allValuesFrom rdf:resource="http://eao.onl/ontologies/eao.owl#blue"/>
            </owl:Restriction>
        </rdfs:subClassOf>
        <dc:source xml:lang="en">https://pubs.opengroup.org/architecture/archimate3-doc/chap02.html</dc:source>
        <rdfs:comment xml:lang="en">depicts application services that support the business, and the applications that realize them</rdfs:comment>
        <rdfs:label xml:lang="en">application layer</rdfs:label>
    </owl:Class>
    


    <!-- http://eao.onl/ontologies/eao.owl#architecture -->

    <owl:Class rdf:about="http://eao.onl/ontologies/eao.owl#architecture">
        <rdfs:subClassOf rdf:resource="http://purl.obolibrary.org/obo/BFO_0000004"/>
        <rdfs:subClassOf>
            <owl:Restriction>
                <owl:onProperty rdf:resource="http://purl.obolibrary.org/obo/RO_0001019"/>
                <owl:someValuesFrom rdf:resource="http://eao.onl/ontologies/eao.owl#architecture_view"/>
            </owl:Restriction>
        </rdfs:subClassOf>
        <rdfs:subClassOf>
            <owl:Restriction>
                <owl:onProperty rdf:resource="http://purl.obolibrary.org/obo/RO_0001019"/>
                <owl:someValuesFrom rdf:resource="http://eao.onl/ontologies/eao.owl#element"/>
            </owl:Restriction>
        </rdfs:subClassOf>
        <rdfs:subClassOf>
            <owl:Restriction>
                <owl:onProperty rdf:resource="http://purl.obolibrary.org/obo/RO_0001019"/>
                <owl:someValuesFrom rdf:resource="http://eao.onl/ontologies/eao.owl#layer"/>
            </owl:Restriction>
        </rdfs:subClassOf>
        <rdfs:comment xml:lang="en">The fundamental concepts or properties of a system in its environment embodied in its elements, relationships, and in pricinples of its design and evolution.

[Source: ISO/IEC/IEEE 42010:2011]

The structure of components, their inter-relationships, and the principles and guidelines governing their designs and evolution over time.

[Source: TOGAF 9 addition]</rdfs:comment>
        <rdfs:label xml:lang="en">architecture</rdfs:label>
    </owl:Class>
    


    <!-- http://eao.onl/ontologies/eao.owl#architecture_view -->

    <owl:Class rdf:about="http://eao.onl/ontologies/eao.owl#architecture_view">
        <rdfs:subClassOf rdf:resource="http://purl.obolibrary.org/obo/BFO_0000004"/>
        <dc:source xml:lang="en">https://pubs.opengroup.org/architecture/archimate3-doc/chap02.html</dc:source>
        <rdfs:comment xml:lang="en">A representation of a system from the perspective of a related set of concerns.

[Source: Archimate 3.1]</rdfs:comment>
        <rdfs:label xml:lang="en">architecture view</rdfs:label>
        <rdfs:label xml:lang="en">view</rdfs:label>
    </owl:Class>
    


    <!-- http://eao.onl/ontologies/eao.owl#architecture_viewpoint -->

    <owl:Class rdf:about="http://eao.onl/ontologies/eao.owl#architecture_viewpoint">
        <rdfs:subClassOf rdf:resource="http://purl.obolibrary.org/obo/BFO_0000004"/>
        <dc:source xml:lang="en">https://pubs.opengroup.org/architecture/archimate3-doc/chap02.html</dc:source>
        <CommonCoreOntologies:alternative_label xml:lang="en">viewpoint</CommonCoreOntologies:alternative_label>
        <rdfs:comment>A specification of the conventions for a particular kind of architecture view.

[Source: Archimate 3.1]</rdfs:comment>
        <rdfs:label xml:lang="en">architecture viewpoint</rdfs:label>
    </owl:Class>
    


    <!-- http://eao.onl/ontologies/eao.owl#aspect -->

    <owl:Class rdf:about="http://eao.onl/ontologies/eao.owl#aspect">
        <rdfs:subClassOf rdf:resource="http://purl.obolibrary.org/obo/BFO_0000004"/>
        <rdfs:subClassOf>
            <owl:Restriction>
                <owl:onProperty rdf:resource="http://eao.onl/ontologies/eao.owl#hasConventionColor"/>
                <owl:someValuesFrom rdf:resource="http://eao.onl/ontologies/eao.owl#aspect_color"/>
            </owl:Restriction>
        </rdfs:subClassOf>
        <dc:source xml:lang="en">https://pubs.opengroup.org/architecture/archimate3-doc/chap02.html</dc:source>
        <rdfs:comment xml:lang="en">Classification of elements based on layer-independent characteristics related to the concerns of different stakeholders. Used for positioning elements in the ArchiMate metamodel.</rdfs:comment>
        <rdfs:label xml:lang="en">aspect</rdfs:label>
    </owl:Class>
    


    <!-- http://eao.onl/ontologies/eao.owl#aspect_color -->

    <owl:Class rdf:about="http://eao.onl/ontologies/eao.owl#aspect_color">
        <rdfs:subClassOf rdf:resource="http://eao.onl/ontologies/eao.owl#color"/>
        <owl:disjointWith rdf:resource="http://eao.onl/ontologies/eao.owl#layer_color"/>
        <rdfs:comment xml:lang="en">shades of grey are used to distinguish elements belonging to the different aspects of the ArchiMate framework</rdfs:comment>
    </owl:Class>
    


    <!-- http://eao.onl/ontologies/eao.owl#behavior_aspect -->

    <owl:Class rdf:about="http://eao.onl/ontologies/eao.owl#behavior_aspect">
        <rdfs:subClassOf rdf:resource="http://eao.onl/ontologies/eao.owl#aspect"/>
        <rdfs:subClassOf>
            <owl:Restriction>
                <owl:onProperty rdf:resource="http://eao.onl/ontologies/eao.owl#hasConventionColor"/>
                <owl:allValuesFrom rdf:resource="http://eao.onl/ontologies/eao.owl#medium_grey"/>
            </owl:Restriction>
        </rdfs:subClassOf>
        <dc:source xml:lang="en">https://pubs.opengroup.org/architecture/archimate3-doc/chap03.html</dc:source>
        <rdfs:comment xml:lang="en">represents the behavior (processes, functions, events, and services) performed by the actors; structural elements are assigned to behavioral elements, to show who or what displays the behavior</rdfs:comment>
        <rdfs:label xml:lang="en">behavior aspect</rdfs:label>
    </owl:Class>
    


    <!-- http://eao.onl/ontologies/eao.owl#behavior_element -->

    <owl:Class rdf:about="http://eao.onl/ontologies/eao.owl#behavior_element">
        <rdfs:subClassOf rdf:resource="http://eao.onl/ontologies/eao.owl#element"/>
        <dc:source xml:lang="en">https://pubs.opengroup.org/architecture/archimate3-doc/chap04.html</dc:source>
        <rdfs:label xml:lang="en">behavior element</rdfs:label>
    </owl:Class>
    


    <!-- http://eao.onl/ontologies/eao.owl#blue -->

    <owl:Class rdf:about="http://eao.onl/ontologies/eao.owl#blue">
        <rdfs:subClassOf rdf:resource="http://eao.onl/ontologies/eao.owl#layer_color"/>
    </owl:Class>
    


    <!-- http://eao.onl/ontologies/eao.owl#business_layer -->

    <owl:Class rdf:about="http://eao.onl/ontologies/eao.owl#business_layer">
        <rdfs:subClassOf rdf:resource="http://eao.onl/ontologies/eao.owl#layer"/>
        <rdfs:subClassOf>
            <owl:Restriction>
                <owl:onProperty rdf:resource="http://eao.onl/ontologies/eao.owl#hasConventionColor"/>
                <owl:allValuesFrom rdf:resource="http://eao.onl/ontologies/eao.owl#yellow"/>
            </owl:Restriction>
        </rdfs:subClassOf>
        <dc:source xml:lang="en">https://pubs.opengroup.org/architecture/archimate3-doc/chap02.html</dc:source>
        <rdfs:comment xml:lang="en">depicts business services offered to customers, which are realized in the organization by business processes performed by business actors</rdfs:comment>
        <rdfs:label xml:lang="en">business layer</rdfs:label>
    </owl:Class>
    


    <!-- http://eao.onl/ontologies/eao.owl#collaboration -->

    <owl:Class rdf:about="http://eao.onl/ontologies/eao.owl#collaboration">
        <rdfs:subClassOf rdf:resource="http://eao.onl/ontologies/eao.owl#internal_active_structure_element"/>
        <rdfs:subClassOf>
            <owl:Restriction>
                <owl:onProperty rdf:resource="http://eao.onl/ontologies/eao.owl#aggregates"/>
                <owl:minQualifiedCardinality rdf:datatype="http://www.w3.org/2001/XMLSchema#nonNegativeInteger">2</owl:minQualifiedCardinality>
                <owl:onClass rdf:resource="http://eao.onl/ontologies/eao.owl#internal_active_structure_element"/>
            </owl:Restriction>
        </rdfs:subClassOf>
        <dc:source xml:lang="en">https://pubs.opengroup.org/architecture/archimate3-doc/chap04.html</dc:source>
        <rdfs:comment xml:lang="en">Represents an aggregate of two or more internal active structure elements, working together to perform some collective behavior.</rdfs:comment>
        <rdfs:label xml:lang="en">collaboration</rdfs:label>
    </owl:Class>
    


    <!-- http://eao.onl/ontologies/eao.owl#color -->

    <owl:Class rdf:about="http://eao.onl/ontologies/eao.owl#color">
        <rdfs:subClassOf rdf:resource="http://purl.obolibrary.org/obo/BFO_0000019"/>
        <rdfs:comment xml:lang="en">convention colors, used to distinguish between the layers and aspects of the Archimate Core Framework</rdfs:comment>
        <rdfs:label xml:lang="en">color</rdfs:label>
    </owl:Class>
    


    <!-- http://eao.onl/ontologies/eao.owl#composite_element -->

    <owl:Class rdf:about="http://eao.onl/ontologies/eao.owl#composite_element">
        <rdfs:subClassOf rdf:resource="http://eao.onl/ontologies/eao.owl#element"/>
        <rdfs:subClassOf>
            <owl:Restriction>
                <owl:onProperty rdf:resource="http://eao.onl/ontologies/eao.owl#aggregates"/>
                <owl:someValuesFrom rdf:resource="http://eao.onl/ontologies/eao.owl#composite_element"/>
            </owl:Restriction>
        </rdfs:subClassOf>
        <rdfs:subClassOf>
            <owl:Restriction>
                <owl:onProperty rdf:resource="http://eao.onl/ontologies/eao.owl#hasSpecialization"/>
                <owl:someValuesFrom rdf:resource="http://eao.onl/ontologies/eao.owl#grouping"/>
            </owl:Restriction>
        </rdfs:subClassOf>
        <rdfs:subClassOf>
            <owl:Restriction>
                <owl:onProperty rdf:resource="http://eao.onl/ontologies/eao.owl#hasSpecialization"/>
                <owl:someValuesFrom rdf:resource="http://eao.onl/ontologies/eao.owl#location"/>
            </owl:Restriction>
        </rdfs:subClassOf>
        <rdfs:subClassOf>
            <owl:Restriction>
                <owl:onProperty rdf:resource="http://eao.onl/ontologies/eao.owl#isComposedOf"/>
                <owl:someValuesFrom rdf:resource="http://eao.onl/ontologies/eao.owl#composite_element"/>
            </owl:Restriction>
        </rdfs:subClassOf>
        <dc:source xml:lang="en">https://pubs.opengroup.org/architecture/archimate3-doc/chap02.html</dc:source>
        <rdfs:comment xml:lang="en">an element consisting of other elements from multiple aspects or layers of the language</rdfs:comment>
        <rdfs:label xml:lang="en">composite element</rdfs:label>
    </owl:Class>
    


    <!-- http://eao.onl/ontologies/eao.owl#corner_shape -->

    <owl:Class rdf:about="http://eao.onl/ontologies/eao.owl#corner_shape">
        <rdfs:subClassOf rdf:resource="http://purl.obolibrary.org/obo/BFO_0000019"/>
        <rdfs:subClassOf>
            <owl:Restriction>
                <owl:onProperty rdf:resource="http://eao.onl/ontologies/eao.owl#accesses"/>
                <owl:someValuesFrom rdf:resource="http://eao.onl/ontologies/eao.owl#passive_structure_element"/>
            </owl:Restriction>
        </rdfs:subClassOf>
        <rdfs:subClassOf>
            <owl:Restriction>
                <owl:onProperty rdf:resource="http://eao.onl/ontologies/eao.owl#aggregates"/>
                <owl:someValuesFrom rdf:resource="http://eao.onl/ontologies/eao.owl#internal_behavior_element"/>
            </owl:Restriction>
        </rdfs:subClassOf>
        <rdfs:subClassOf>
            <owl:Restriction>
                <owl:onProperty rdf:resource="http://eao.onl/ontologies/eao.owl#flowsTo"/>
                <owl:someValuesFrom rdf:resource="http://eao.onl/ontologies/eao.owl#event"/>
            </owl:Restriction>
        </rdfs:subClassOf>
        <rdfs:subClassOf>
            <owl:Restriction>
                <owl:onProperty rdf:resource="http://eao.onl/ontologies/eao.owl#flowsTo"/>
                <owl:someValuesFrom rdf:resource="http://eao.onl/ontologies/eao.owl#internal_behavior_element"/>
            </owl:Restriction>
        </rdfs:subClassOf>
        <rdfs:subClassOf>
            <owl:Restriction>
                <owl:onProperty rdf:resource="http://eao.onl/ontologies/eao.owl#isComposedOf"/>
                <owl:someValuesFrom rdf:resource="http://eao.onl/ontologies/eao.owl#internal_behavior_element"/>
            </owl:Restriction>
        </rdfs:subClassOf>
        <rdfs:subClassOf>
            <owl:Restriction>
                <owl:onProperty rdf:resource="http://eao.onl/ontologies/eao.owl#triggers"/>
                <owl:someValuesFrom rdf:resource="http://eao.onl/ontologies/eao.owl#event"/>
            </owl:Restriction>
        </rdfs:subClassOf>
        <rdfs:subClassOf>
            <owl:Restriction>
                <owl:onProperty rdf:resource="http://eao.onl/ontologies/eao.owl#triggers"/>
                <owl:someValuesFrom rdf:resource="http://eao.onl/ontologies/eao.owl#internal_behavior_element"/>
            </owl:Restriction>
        </rdfs:subClassOf>
    </owl:Class>
    


    <!-- http://eao.onl/ontologies/eao.owl#dark_green -->

    <owl:Class rdf:about="http://eao.onl/ontologies/eao.owl#dark_green">
        <rdfs:subClassOf rdf:resource="http://eao.onl/ontologies/eao.owl#layer_color"/>
    </owl:Class>
    


    <!-- http://eao.onl/ontologies/eao.owl#dark_grey -->

    <owl:Class rdf:about="http://eao.onl/ontologies/eao.owl#dark_grey">
        <rdfs:subClassOf rdf:resource="http://eao.onl/ontologies/eao.owl#aspect_color"/>
    </owl:Class>
    


    <!-- http://eao.onl/ontologies/eao.owl#diagonal_corners -->

    <owl:Class rdf:about="http://eao.onl/ontologies/eao.owl#diagonal_corners">
        <rdfs:subClassOf rdf:resource="http://eao.onl/ontologies/eao.owl#corner_shape"/>
    </owl:Class>
    


    <!-- http://eao.onl/ontologies/eao.owl#element -->

    <owl:Class rdf:about="http://eao.onl/ontologies/eao.owl#element">
        <rdfs:subClassOf rdf:resource="http://purl.obolibrary.org/obo/BFO_0000004"/>
        <rdfs:subClassOf>
            <owl:Restriction>
                <owl:onProperty rdf:resource="http://eao.onl/ontologies/eao.owl#hasConventionShape"/>
                <owl:someValuesFrom rdf:resource="http://eao.onl/ontologies/eao.owl#corner_shape"/>
            </owl:Restriction>
        </rdfs:subClassOf>
        <rdfs:subClassOf>
            <owl:Restriction>
                <owl:onProperty rdf:resource="http://purl.obolibrary.org/obo/RO_0001025"/>
                <owl:someValuesFrom rdf:resource="http://eao.onl/ontologies/eao.owl#location"/>
            </owl:Restriction>
        </rdfs:subClassOf>
        <dc:source xml:lang="en">https://pubs.opengroup.org/architecture/archimate3-doc/chap02.html</dc:source>
        <rdfs:comment xml:lang="en">Basic unit, used to define and describe the constituent parts of Enterprise Architectures and their unique set of characteristics</rdfs:comment>
        <rdfs:label xml:lang="en">element</rdfs:label>
    </owl:Class>
    


    <!-- http://eao.onl/ontologies/eao.owl#enterprise -->

    <owl:Class rdf:about="http://eao.onl/ontologies/eao.owl#enterprise">
        <rdfs:subClassOf rdf:resource="http://purl.obolibrary.org/obo/BFO_0000004"/>
        <rdfs:subClassOf>
            <owl:Restriction>
                <owl:onProperty rdf:resource="http://eao.onl/ontologies/eao.owl#hasArchitecture"/>
                <owl:someValuesFrom rdf:resource="http://eao.onl/ontologies/eao.owl#enterprise_architecture"/>
            </owl:Restriction>
        </rdfs:subClassOf>
        <obo:IAO_0000112 xml:lang="en">a chain of geographically distant organisations linked together by common ownership</obo:IAO_0000112>
        <obo:IAO_0000112 xml:lang="en">a division of a corporation</obo:IAO_0000112>
        <obo:IAO_0000112 xml:lang="en">a government agency</obo:IAO_0000112>
        <obo:IAO_0000112 xml:lang="en">a single government department</obo:IAO_0000112>
        <obo:IAO_0000112 xml:lang="en">a whole corporation</obo:IAO_0000112>
        <obo:IAO_0000112 xml:lang="en">groups of countries or governments working together to create common or shareable deliverables or infrastructure</obo:IAO_0000112>
        <obo:IAO_0000112 xml:lang="en">partnerships and alliances of businesses working together</obo:IAO_0000112>
        <rdfs:comment xml:lang="en">An enterprise is any collection of organisations that has common goals

[Source: TOGAF 9]</rdfs:comment>
        <rdfs:label xml:lang="en">enterprise</rdfs:label>
    </owl:Class>
    


    <!-- http://eao.onl/ontologies/eao.owl#enterprise_architecture -->

    <owl:Class rdf:about="http://eao.onl/ontologies/eao.owl#enterprise_architecture">
        <rdfs:subClassOf rdf:resource="http://eao.onl/ontologies/eao.owl#architecture"/>
        <rdfs:comment xml:lang="en">The organising logic for business processes and IT infrastructure reflecting the integration and standardising requirements of the firm&apos;s operating model.

[Source: MIT Center for Information Systems Research]</rdfs:comment>
        <rdfs:label xml:lang="en">enterprise architecture</rdfs:label>
    </owl:Class>
    


    <!-- http://eao.onl/ontologies/eao.owl#event -->

    <owl:Class rdf:about="http://eao.onl/ontologies/eao.owl#event">
        <owl:equivalentClass>
            <owl:Class>
                <owl:unionOf rdf:parseType="Collection">
                    <rdf:Description rdf:about="http://www.ontologyrepository.com/CommonCoreOntologies/Act"/>
                    <rdf:Description rdf:about="http://www.ontologyrepository.com/CommonCoreOntologies/Change"/>
                </owl:unionOf>
            </owl:Class>
        </owl:equivalentClass>
        <rdfs:subClassOf rdf:resource="http://eao.onl/ontologies/eao.owl#behavior_element"/>
        <rdfs:subClassOf>
            <owl:Restriction>
                <owl:onProperty rdf:resource="http://eao.onl/ontologies/eao.owl#accesses"/>
                <owl:someValuesFrom rdf:resource="http://eao.onl/ontologies/eao.owl#passive_structure_element"/>
            </owl:Restriction>
        </rdfs:subClassOf>
        <rdfs:subClassOf>
            <owl:Restriction>
                <owl:onProperty rdf:resource="http://eao.onl/ontologies/eao.owl#aggregates"/>
                <owl:someValuesFrom rdf:resource="http://eao.onl/ontologies/eao.owl#event"/>
            </owl:Restriction>
        </rdfs:subClassOf>
        <rdfs:subClassOf>
            <owl:Restriction>
                <owl:onProperty rdf:resource="http://eao.onl/ontologies/eao.owl#flowsTo"/>
                <owl:someValuesFrom rdf:resource="http://eao.onl/ontologies/eao.owl#event"/>
            </owl:Restriction>
        </rdfs:subClassOf>
        <rdfs:subClassOf>
            <owl:Restriction>
                <owl:onProperty rdf:resource="http://eao.onl/ontologies/eao.owl#flowsTo"/>
                <owl:someValuesFrom rdf:resource="http://eao.onl/ontologies/eao.owl#external_behavior_element"/>
            </owl:Restriction>
        </rdfs:subClassOf>
        <rdfs:subClassOf>
            <owl:Restriction>
                <owl:onProperty rdf:resource="http://eao.onl/ontologies/eao.owl#flowsTo"/>
                <owl:someValuesFrom rdf:resource="http://eao.onl/ontologies/eao.owl#internal_behavior_element"/>
            </owl:Restriction>
        </rdfs:subClassOf>
        <rdfs:subClassOf>
            <owl:Restriction>
                <owl:onProperty rdf:resource="http://eao.onl/ontologies/eao.owl#hasSpecialization"/>
                <owl:someValuesFrom rdf:resource="http://eao.onl/ontologies/eao.owl#event"/>
            </owl:Restriction>
        </rdfs:subClassOf>
        <rdfs:subClassOf>
            <owl:Restriction>
                <owl:onProperty rdf:resource="http://eao.onl/ontologies/eao.owl#isComposedOf"/>
                <owl:someValuesFrom rdf:resource="http://eao.onl/ontologies/eao.owl#event"/>
            </owl:Restriction>
        </rdfs:subClassOf>
        <rdfs:subClassOf>
            <owl:Restriction>
                <owl:onProperty rdf:resource="http://eao.onl/ontologies/eao.owl#triggers"/>
                <owl:someValuesFrom rdf:resource="http://eao.onl/ontologies/eao.owl#event"/>
            </owl:Restriction>
        </rdfs:subClassOf>
        <rdfs:subClassOf>
            <owl:Restriction>
                <owl:onProperty rdf:resource="http://eao.onl/ontologies/eao.owl#triggers"/>
                <owl:someValuesFrom rdf:resource="http://eao.onl/ontologies/eao.owl#external_behavior_element"/>
            </owl:Restriction>
        </rdfs:subClassOf>
        <rdfs:subClassOf>
            <owl:Restriction>
                <owl:onProperty rdf:resource="http://eao.onl/ontologies/eao.owl#triggers"/>
                <owl:someValuesFrom rdf:resource="http://eao.onl/ontologies/eao.owl#internal_behavior_element"/>
            </owl:Restriction>
        </rdfs:subClassOf>
        <dc:source xml:lang="en">https://pubs.opengroup.org/architecture/archimate3-doc/chap04.html</dc:source>
        <rdfs:comment xml:lang="en">Represents a state change.</rdfs:comment>
        <rdfs:label xml:lang="en">event</rdfs:label>
    </owl:Class>
    


    <!-- http://eao.onl/ontologies/eao.owl#external_active_structure_element -->

    <owl:Class rdf:about="http://eao.onl/ontologies/eao.owl#external_active_structure_element">
        <rdfs:subClassOf rdf:resource="http://eao.onl/ontologies/eao.owl#active_structure_element"/>
        <rdfs:subClassOf>
            <owl:Restriction>
                <owl:onProperty rdf:resource="http://eao.onl/ontologies/eao.owl#aggregates"/>
                <owl:someValuesFrom rdf:resource="http://eao.onl/ontologies/eao.owl#external_active_structure_element"/>
            </owl:Restriction>
        </rdfs:subClassOf>
        <rdfs:subClassOf>
            <owl:Restriction>
                <owl:onProperty rdf:resource="http://eao.onl/ontologies/eao.owl#hasSpecialization"/>
                <owl:someValuesFrom rdf:resource="http://eao.onl/ontologies/eao.owl#external_active_structure_element"/>
            </owl:Restriction>
        </rdfs:subClassOf>
        <rdfs:subClassOf>
            <owl:Restriction>
                <owl:onProperty rdf:resource="http://eao.onl/ontologies/eao.owl#isAssignedTo"/>
                <owl:someValuesFrom rdf:resource="http://eao.onl/ontologies/eao.owl#external_behavior_element"/>
            </owl:Restriction>
        </rdfs:subClassOf>
        <rdfs:subClassOf>
            <owl:Restriction>
                <owl:onProperty rdf:resource="http://eao.onl/ontologies/eao.owl#isComposedOf"/>
                <owl:someValuesFrom rdf:resource="http://eao.onl/ontologies/eao.owl#external_active_structure_element"/>
            </owl:Restriction>
        </rdfs:subClassOf>
        <rdfs:subClassOf>
            <owl:Restriction>
                <owl:onProperty rdf:resource="http://eao.onl/ontologies/eao.owl#serves"/>
                <owl:someValuesFrom rdf:resource="http://eao.onl/ontologies/eao.owl#internal_active_structure_element"/>
            </owl:Restriction>
        </rdfs:subClassOf>
        <owl:disjointWith rdf:resource="http://eao.onl/ontologies/eao.owl#internal_active_structure_element"/>
        <dc:source xml:lang="en">https://pubs.opengroup.org/architecture/archimate3-doc/chap04.html</dc:source>
        <CommonCoreOntologies:alternative_label xml:lang="en">interface</CommonCoreOntologies:alternative_label>
        <CommonCoreOntologies:http_query_string xml:lang="en">https://pubs.opengroup.org/architecture/archimate3-doc/chap04.html</CommonCoreOntologies:http_query_string>
        <rdfs:comment xml:lang="en">Represents a point of access where one or more services are exposed to the environment.</rdfs:comment>
        <rdfs:label xml:lang="en">external active structure element</rdfs:label>
    </owl:Class>
    


    <!-- http://eao.onl/ontologies/eao.owl#external_behavior_element -->

    <owl:Class rdf:about="http://eao.onl/ontologies/eao.owl#external_behavior_element">
        <rdfs:subClassOf rdf:resource="http://eao.onl/ontologies/eao.owl#behavior_element"/>
        <rdfs:subClassOf>
            <owl:Restriction>
                <owl:onProperty rdf:resource="http://eao.onl/ontologies/eao.owl#accesses"/>
                <owl:someValuesFrom rdf:resource="http://eao.onl/ontologies/eao.owl#passive_structure_element"/>
            </owl:Restriction>
        </rdfs:subClassOf>
        <rdfs:subClassOf>
            <owl:Restriction>
                <owl:onProperty rdf:resource="http://eao.onl/ontologies/eao.owl#aggregates"/>
                <owl:someValuesFrom rdf:resource="http://eao.onl/ontologies/eao.owl#external_behavior_element"/>
            </owl:Restriction>
        </rdfs:subClassOf>
        <rdfs:subClassOf>
            <owl:Restriction>
                <owl:onProperty rdf:resource="http://eao.onl/ontologies/eao.owl#flowsTo"/>
                <owl:someValuesFrom rdf:resource="http://eao.onl/ontologies/eao.owl#event"/>
            </owl:Restriction>
        </rdfs:subClassOf>
        <rdfs:subClassOf>
            <owl:Restriction>
                <owl:onProperty rdf:resource="http://eao.onl/ontologies/eao.owl#flowsTo"/>
                <owl:someValuesFrom rdf:resource="http://eao.onl/ontologies/eao.owl#external_behavior_element"/>
            </owl:Restriction>
        </rdfs:subClassOf>
        <rdfs:subClassOf>
            <owl:Restriction>
                <owl:onProperty rdf:resource="http://eao.onl/ontologies/eao.owl#hasSpecialization"/>
                <owl:someValuesFrom rdf:resource="http://eao.onl/ontologies/eao.owl#external_behavior_element"/>
            </owl:Restriction>
        </rdfs:subClassOf>
        <rdfs:subClassOf>
            <owl:Restriction>
                <owl:onProperty rdf:resource="http://eao.onl/ontologies/eao.owl#isComposedOf"/>
                <owl:someValuesFrom rdf:resource="http://eao.onl/ontologies/eao.owl#external_behavior_element"/>
            </owl:Restriction>
        </rdfs:subClassOf>
        <rdfs:subClassOf>
            <owl:Restriction>
                <owl:onProperty rdf:resource="http://eao.onl/ontologies/eao.owl#serves"/>
                <owl:someValuesFrom rdf:resource="http://eao.onl/ontologies/eao.owl#internal_active_structure_element"/>
            </owl:Restriction>
        </rdfs:subClassOf>
        <rdfs:subClassOf>
            <owl:Restriction>
                <owl:onProperty rdf:resource="http://eao.onl/ontologies/eao.owl#serves"/>
                <owl:someValuesFrom rdf:resource="http://eao.onl/ontologies/eao.owl#internal_behavior_element"/>
            </owl:Restriction>
        </rdfs:subClassOf>
        <rdfs:subClassOf>
            <owl:Restriction>
                <owl:onProperty rdf:resource="http://eao.onl/ontologies/eao.owl#triggers"/>
                <owl:someValuesFrom rdf:resource="http://eao.onl/ontologies/eao.owl#event"/>
            </owl:Restriction>
        </rdfs:subClassOf>
        <rdfs:subClassOf>
            <owl:Restriction>
                <owl:onProperty rdf:resource="http://eao.onl/ontologies/eao.owl#triggers"/>
                <owl:someValuesFrom rdf:resource="http://eao.onl/ontologies/eao.owl#external_behavior_element"/>
            </owl:Restriction>
        </rdfs:subClassOf>
        <dc:source xml:lang="en">https://pubs.opengroup.org/architecture/archimate3-doc/chap04.html</dc:source>
        <CommonCoreOntologies:alternative_label xml:lang="en">service</CommonCoreOntologies:alternative_label>
        <rdfs:comment xml:lang="en">Represents an explicitly defined exposed behavior.</rdfs:comment>
        <rdfs:label xml:lang="en">external behavior element</rdfs:label>
    </owl:Class>
    


    <!-- http://eao.onl/ontologies/eao.owl#green -->

    <owl:Class rdf:about="http://eao.onl/ontologies/eao.owl#green">
        <rdfs:subClassOf rdf:resource="http://eao.onl/ontologies/eao.owl#layer_color"/>
    </owl:Class>
    


    <!-- http://eao.onl/ontologies/eao.owl#grouping -->

    <owl:Class rdf:about="http://eao.onl/ontologies/eao.owl#grouping">
        <rdfs:subClassOf rdf:resource="http://purl.obolibrary.org/obo/BFO_0000004"/>
        <rdfs:subClassOf>
            <owl:Restriction>
                <owl:onProperty rdf:resource="http://purl.obolibrary.org/obo/RO_0001019"/>
                <owl:someValuesFrom rdf:resource="http://eao.onl/ontologies/eao.owl#element"/>
            </owl:Restriction>
        </rdfs:subClassOf>
        <owl:disjointWith rdf:resource="http://eao.onl/ontologies/eao.owl#location"/>
        <dc:source xml:lang="en">https://pubs.opengroup.org/architecture/archimate3-doc/chap04.html</dc:source>
        <rdfs:comment xml:lang="en">aggregates or composes concepts that belong together based on some common characteristic.</rdfs:comment>
        <rdfs:label xml:lang="en">grouping</rdfs:label>
    </owl:Class>
    


    <!-- http://eao.onl/ontologies/eao.owl#interaction -->

    <owl:Class rdf:about="http://eao.onl/ontologies/eao.owl#interaction">
        <rdfs:subClassOf rdf:resource="http://eao.onl/ontologies/eao.owl#internal_behavior_element"/>
        <dc:source xml:lang="en">https://pubs.opengroup.org/architecture/archimate3-doc/chap04.html</dc:source>
        <rdfs:comment xml:lang="en">Represents a unit of collective behavior that must be performed by two or more internal active structure elements, either assigned directly or aggregated in a collaboration.</rdfs:comment>
        <rdfs:label xml:lang="en">interaction</rdfs:label>
    </owl:Class>
    


    <!-- http://eao.onl/ontologies/eao.owl#internal_active_structure_element -->

    <owl:Class rdf:about="http://eao.onl/ontologies/eao.owl#internal_active_structure_element">
        <rdfs:subClassOf rdf:resource="http://eao.onl/ontologies/eao.owl#active_structure_element"/>
        <rdfs:subClassOf>
            <owl:Restriction>
                <owl:onProperty rdf:resource="http://eao.onl/ontologies/eao.owl#aggregates"/>
                <owl:someValuesFrom rdf:resource="http://eao.onl/ontologies/eao.owl#internal_active_structure_element"/>
            </owl:Restriction>
        </rdfs:subClassOf>
        <rdfs:subClassOf>
            <owl:Restriction>
                <owl:onProperty rdf:resource="http://eao.onl/ontologies/eao.owl#hasSpecialization"/>
                <owl:someValuesFrom rdf:resource="http://eao.onl/ontologies/eao.owl#collaboration"/>
            </owl:Restriction>
        </rdfs:subClassOf>
        <rdfs:subClassOf>
            <owl:Restriction>
                <owl:onProperty rdf:resource="http://eao.onl/ontologies/eao.owl#hasSpecialization"/>
                <owl:someValuesFrom rdf:resource="http://eao.onl/ontologies/eao.owl#internal_active_structure_element"/>
            </owl:Restriction>
        </rdfs:subClassOf>
        <rdfs:subClassOf>
            <owl:Restriction>
                <owl:onProperty rdf:resource="http://eao.onl/ontologies/eao.owl#isAssignedTo"/>
                <owl:someValuesFrom rdf:resource="http://eao.onl/ontologies/eao.owl#internal_behavior_element"/>
            </owl:Restriction>
        </rdfs:subClassOf>
        <rdfs:subClassOf>
            <owl:Restriction>
                <owl:onProperty rdf:resource="http://eao.onl/ontologies/eao.owl#isComposedOf"/>
                <owl:someValuesFrom rdf:resource="http://eao.onl/ontologies/eao.owl#external_active_structure_element"/>
            </owl:Restriction>
        </rdfs:subClassOf>
        <rdfs:subClassOf>
            <owl:Restriction>
                <owl:onProperty rdf:resource="http://eao.onl/ontologies/eao.owl#isComposedOf"/>
                <owl:someValuesFrom rdf:resource="http://eao.onl/ontologies/eao.owl#internal_active_structure_element"/>
            </owl:Restriction>
        </rdfs:subClassOf>
        <dc:source xml:lang="en">https://pubs.opengroup.org/architecture/archimate3-doc/chap04.html</dc:source>
        <rdfs:comment xml:lang="en">Represents an entity that is capable of performing behavior.</rdfs:comment>
        <rdfs:label xml:lang="en">internal active structure element</rdfs:label>
    </owl:Class>
    


    <!-- http://eao.onl/ontologies/eao.owl#internal_behavior_element -->

    <owl:Class rdf:about="http://eao.onl/ontologies/eao.owl#internal_behavior_element">
        <rdfs:subClassOf rdf:resource="http://eao.onl/ontologies/eao.owl#behavior_element"/>
        <rdfs:subClassOf>
            <owl:Restriction>
                <owl:onProperty rdf:resource="http://eao.onl/ontologies/eao.owl#accesses"/>
                <owl:someValuesFrom rdf:resource="http://eao.onl/ontologies/eao.owl#passive_structure_element"/>
            </owl:Restriction>
        </rdfs:subClassOf>
        <rdfs:subClassOf>
            <owl:Restriction>
                <owl:onProperty rdf:resource="http://eao.onl/ontologies/eao.owl#aggregates"/>
                <owl:someValuesFrom rdf:resource="http://eao.onl/ontologies/eao.owl#internal_behavior_element"/>
            </owl:Restriction>
        </rdfs:subClassOf>
        <rdfs:subClassOf>
            <owl:Restriction>
                <owl:onProperty rdf:resource="http://eao.onl/ontologies/eao.owl#flowsTo"/>
                <owl:someValuesFrom rdf:resource="http://eao.onl/ontologies/eao.owl#event"/>
            </owl:Restriction>
        </rdfs:subClassOf>
        <rdfs:subClassOf>
            <owl:Restriction>
                <owl:onProperty rdf:resource="http://eao.onl/ontologies/eao.owl#flowsTo"/>
                <owl:someValuesFrom rdf:resource="http://eao.onl/ontologies/eao.owl#internal_behavior_element"/>
            </owl:Restriction>
        </rdfs:subClassOf>
        <rdfs:subClassOf>
            <owl:Restriction>
                <owl:onProperty rdf:resource="http://eao.onl/ontologies/eao.owl#hasSpecialization"/>
                <owl:someValuesFrom rdf:resource="http://eao.onl/ontologies/eao.owl#internal_behavior_element"/>
            </owl:Restriction>
        </rdfs:subClassOf>
        <rdfs:subClassOf>
            <owl:Restriction>
                <owl:onProperty rdf:resource="http://eao.onl/ontologies/eao.owl#isComposedOf"/>
                <owl:someValuesFrom rdf:resource="http://eao.onl/ontologies/eao.owl#internal_behavior_element"/>
            </owl:Restriction>
        </rdfs:subClassOf>
        <rdfs:subClassOf>
            <owl:Restriction>
                <owl:onProperty rdf:resource="http://eao.onl/ontologies/eao.owl#triggers"/>
                <owl:someValuesFrom rdf:resource="http://eao.onl/ontologies/eao.owl#event"/>
            </owl:Restriction>
        </rdfs:subClassOf>
        <rdfs:subClassOf>
            <owl:Restriction>
                <owl:onProperty rdf:resource="http://eao.onl/ontologies/eao.owl#triggers"/>
                <owl:someValuesFrom rdf:resource="http://eao.onl/ontologies/eao.owl#internal_behavior_element"/>
            </owl:Restriction>
        </rdfs:subClassOf>
        <rdfs:subClassOf>
            <owl:Restriction>
                <owl:onProperty rdf:resource="http://purl.obolibrary.org/obo/BFO_0000055"/>
                <owl:someValuesFrom rdf:resource="http://eao.onl/ontologies/eao.owl#external_behavior_element"/>
            </owl:Restriction>
        </rdfs:subClassOf>
        <dc:source xml:lang="en">https://pubs.opengroup.org/architecture/archimate3-doc/chap04.html</dc:source>
        <rdfs:comment xml:lang="en">An internal behavior element represents a unit of activity that can be performed by one or more active structure elements.</rdfs:comment>
        <rdfs:label xml:lang="en">internal behavior element</rdfs:label>
    </owl:Class>
    


    <!-- http://eao.onl/ontologies/eao.owl#layer -->

    <owl:Class rdf:about="http://eao.onl/ontologies/eao.owl#layer">
        <rdfs:subClassOf rdf:resource="http://purl.obolibrary.org/obo/BFO_0000004"/>
        <rdfs:subClassOf>
            <owl:Restriction>
                <owl:onProperty rdf:resource="http://eao.onl/ontologies/eao.owl#hasConventionColor"/>
                <owl:someValuesFrom rdf:resource="http://eao.onl/ontologies/eao.owl#layer_color"/>
            </owl:Restriction>
        </rdfs:subClassOf>
        <dc:source xml:lang="en">https://pubs.opengroup.org/architecture/archimate3-doc/chap02.html</dc:source>
        <rdfs:comment xml:lang="en">An abstraction of the Archimate framework at which an enterprise can be modeled.

[Source: Archimate 3.1]</rdfs:comment>
        <rdfs:label>layer</rdfs:label>
    </owl:Class>
    


    <!-- http://eao.onl/ontologies/eao.owl#layer_color -->

    <owl:Class rdf:about="http://eao.onl/ontologies/eao.owl#layer_color">
        <rdfs:subClassOf rdf:resource="http://eao.onl/ontologies/eao.owl#color"/>
        <rdfs:comment xml:lang="en">layer colors are used to distinguish between the layers of the ArchiMate Core Framework</rdfs:comment>
    </owl:Class>
    


    <!-- http://eao.onl/ontologies/eao.owl#light_grey -->

    <owl:Class rdf:about="http://eao.onl/ontologies/eao.owl#light_grey">
        <rdfs:subClassOf rdf:resource="http://eao.onl/ontologies/eao.owl#aspect_color"/>
    </owl:Class>
    


    <!-- http://eao.onl/ontologies/eao.owl#location -->

    <owl:Class rdf:about="http://eao.onl/ontologies/eao.owl#location">
        <rdfs:subClassOf rdf:resource="http://purl.obolibrary.org/obo/BFO_0000004"/>
        <rdfs:subClassOf>
            <owl:Restriction>
                <owl:onProperty rdf:resource="http://purl.obolibrary.org/obo/RO_0001015"/>
                <owl:someValuesFrom rdf:resource="http://eao.onl/ontologies/eao.owl#element"/>
            </owl:Restriction>
        </rdfs:subClassOf>
        <dc:source xml:lang="en">https://pubs.opengroup.org/architecture/archimate3-doc/chap04.html</dc:source>
        <rdfs:comment xml:lang="en">Represents a conceptual or physical place or position where concepts are located (e.g., structure elements) or performed (e.g., behavior elements).</rdfs:comment>
        <rdfs:label xml:lang="en">location</rdfs:label>
    </owl:Class>
    


    <!-- http://eao.onl/ontologies/eao.owl#medium_grey -->

    <owl:Class rdf:about="http://eao.onl/ontologies/eao.owl#medium_grey">
        <rdfs:subClassOf rdf:resource="http://eao.onl/ontologies/eao.owl#aspect_color"/>
    </owl:Class>
    


    <!-- http://eao.onl/ontologies/eao.owl#motivation_element -->

    <owl:Class rdf:about="http://eao.onl/ontologies/eao.owl#motivation_element">
        <rdfs:subClassOf rdf:resource="http://eao.onl/ontologies/eao.owl#element"/>
        <dc:source xml:lang="en">https://pubs.opengroup.org/architecture/archimate3-doc/chap04.html</dc:source>
        <rdfs:comment xml:lang="en">A motivation element represents the context of or reason behind the architecture of an enterprise.</rdfs:comment>
        <rdfs:label xml:lang="en">motivation element</rdfs:label>
    </owl:Class>
    


    <!-- http://eao.onl/ontologies/eao.owl#passive_structure_aspect -->

    <owl:Class rdf:about="http://eao.onl/ontologies/eao.owl#passive_structure_aspect">
        <rdfs:subClassOf rdf:resource="http://eao.onl/ontologies/eao.owl#aspect"/>
        <rdfs:subClassOf>
            <owl:Restriction>
                <owl:onProperty rdf:resource="http://eao.onl/ontologies/eao.owl#hasConventionColor"/>
                <owl:allValuesFrom rdf:resource="http://eao.onl/ontologies/eao.owl#light_grey"/>
            </owl:Restriction>
        </rdfs:subClassOf>
        <dc:source xml:lang="en">https://pubs.opengroup.org/architecture/archimate3-doc/chap03.html</dc:source>
        <rdfs:comment xml:lang="en">represents the objects on which behavior is performed; these are usually information objects in the Business Layer and data objects in the Application Layer, but they may also be used to represent physical objects</rdfs:comment>
        <rdfs:label xml:lang="en">passive structure aspect</rdfs:label>
    </owl:Class>
    


    <!-- http://eao.onl/ontologies/eao.owl#passive_structure_element -->

    <owl:Class rdf:about="http://eao.onl/ontologies/eao.owl#passive_structure_element">
        <rdfs:subClassOf rdf:resource="http://eao.onl/ontologies/eao.owl#structure_element"/>
        <rdfs:subClassOf>
            <owl:Restriction>
                <owl:onProperty rdf:resource="http://eao.onl/ontologies/eao.owl#aggregates"/>
                <owl:someValuesFrom rdf:resource="http://eao.onl/ontologies/eao.owl#passive_structure_element"/>
            </owl:Restriction>
        </rdfs:subClassOf>
        <rdfs:subClassOf>
            <owl:Restriction>
                <owl:onProperty rdf:resource="http://eao.onl/ontologies/eao.owl#hasSpecialization"/>
                <owl:someValuesFrom rdf:resource="http://eao.onl/ontologies/eao.owl#passive_structure_element"/>
            </owl:Restriction>
        </rdfs:subClassOf>
        <rdfs:subClassOf>
            <owl:Restriction>
                <owl:onProperty rdf:resource="http://eao.onl/ontologies/eao.owl#isComposedOf"/>
                <owl:someValuesFrom rdf:resource="http://eao.onl/ontologies/eao.owl#passive_structure_element"/>
            </owl:Restriction>
        </rdfs:subClassOf>
        <dc:source xml:lang="en">https://pubs.opengroup.org/architecture/archimate3-doc/chap04.html</dc:source>
        <rdfs:comment xml:lang="en">Represents an element on which behavior is performed.</rdfs:comment>
        <rdfs:label xml:lang="en">passive structure element</rdfs:label>
    </owl:Class>
    


    <!-- http://eao.onl/ontologies/eao.owl#round_corners -->

    <owl:Class rdf:about="http://eao.onl/ontologies/eao.owl#round_corners">
        <rdfs:subClassOf rdf:resource="http://eao.onl/ontologies/eao.owl#corner_shape"/>
    </owl:Class>
    


    <!-- http://eao.onl/ontologies/eao.owl#square_corners -->

    <owl:Class rdf:about="http://eao.onl/ontologies/eao.owl#square_corners">
        <rdfs:subClassOf rdf:resource="http://eao.onl/ontologies/eao.owl#corner_shape"/>
    </owl:Class>
    


    <!-- http://eao.onl/ontologies/eao.owl#structure_element -->

    <owl:Class rdf:about="http://eao.onl/ontologies/eao.owl#structure_element">
        <rdfs:subClassOf rdf:resource="http://eao.onl/ontologies/eao.owl#element"/>
        <dc:source xml:lang="en">https://pubs.opengroup.org/architecture/archimate3-doc/chap04.html</dc:source>
        <rdfs:label xml:lang="en">structure element</rdfs:label>
    </owl:Class>
    


    <!-- http://eao.onl/ontologies/eao.owl#technology_layer -->

    <owl:Class rdf:about="http://eao.onl/ontologies/eao.owl#technology_layer">
        <rdfs:subClassOf rdf:resource="http://eao.onl/ontologies/eao.owl#layer"/>
        <rdfs:subClassOf>
            <owl:Restriction>
                <owl:onProperty rdf:resource="http://eao.onl/ontologies/eao.owl#hasConventionColor"/>
                <owl:allValuesFrom rdf:resource="http://eao.onl/ontologies/eao.owl#green"/>
            </owl:Restriction>
        </rdfs:subClassOf>
        <dc:source xml:lang="en">https://pubs.opengroup.org/architecture/archimate3-doc/chap03.html</dc:source>
        <rdfs:comment xml:lang="en">depicts technology services such as processing, storage, and communication services needed to run the applications, and the computer and communication hardware and system software that realize those services. Physical elements are included for modeling physical equipment, materials, and distribution networks to this layer</rdfs:comment>
        <rdfs:label xml:lang="en">technology layer</rdfs:label>
    </owl:Class>
    


    <!-- http://eao.onl/ontologies/eao.owl#white -->

    <owl:Class rdf:about="http://eao.onl/ontologies/eao.owl#white">
        <rdfs:subClassOf rdf:resource="http://eao.onl/ontologies/eao.owl#aspect_color"/>
    </owl:Class>
    


    <!-- http://eao.onl/ontologies/eao.owl#yellow -->

    <owl:Class rdf:about="http://eao.onl/ontologies/eao.owl#yellow">
        <rdfs:subClassOf rdf:resource="http://eao.onl/ontologies/eao.owl#layer_color"/>
    </owl:Class>
    


    <!-- 
    ///////////////////////////////////////////////////////////////////////////////////////
    //
    // General axioms
    //
    ///////////////////////////////////////////////////////////////////////////////////////
     -->

    <rdf:Description>
        <rdf:type rdf:resource="http://www.w3.org/2002/07/owl#AllDisjointClasses"/>
        <owl:members rdf:parseType="Collection">
            <rdf:Description rdf:about="http://eao.onl/ontologies/eao.owl#event"/>
            <rdf:Description rdf:about="http://eao.onl/ontologies/eao.owl#external_behavior_element"/>
            <rdf:Description rdf:about="http://eao.onl/ontologies/eao.owl#internal_behavior_element"/>
        </owl:members>
    </rdf:Description>
</rdf:RDF>



<!-- Generated by the OWL API (version 4.5.9.2019-02-01T07:24:44Z) https://github.com/owlcs/owlapi -->

